Is0/Is0.lean
@@ -9,7 +9,7 @@ import Is0.Programs
 
 namespace Risc0
 
-lemma step_of_sequence_of_assign_eq_state_change :
+lemma Cirgen.step_Sequence_Assign_collapsible :
   ∀ (state : State) (name : String) (op : Op) (program : Cirgen),
   Cirgen.step state (.Sequence (.Assign name op) program) = Cirgen.step (state.update name (Op.eval state op)) program := by
   intros state name op program
@@ -20,12 +20,160 @@ lemma step_of_sequence_of_assign_eq_state_change :
       simp only [State.update, Map.update, beq_iff_eq]
   }
 
+lemma Cirgen.step_Sequence_Set_collapsible
+    {state : State}
+    {name : String}
+    {nameₓ : String}
+    {program : Cirgen}
+    (buffer : List Felt)
+    (x : Felt)
+    (h : state.buffers name = some buffer)
+    (h₁ : state.felts nameₓ = some x) :
+    Cirgen.step state (.Sequence (.Set (Variable.mk name) i (Variable.mk nameₓ)) program)
+  = let buffers' := state.buffers.update name (buffer.set i x)
+    Cirgen.step ({ state with buffers := buffers' }) program := by
+  conv =>
+    lhs
+    unfold step
+  unfold step
+  simp only [Map.update, beq_iff_eq]
+  rw [h]
+  rw [h₁]
+  done
+
+lemma Cirgen.step_Sequence_If_collapsible
+    {state : State}
+    {name : String}
+    {branch : Cirgen}
+    {program : Cirgen}
+    (x : Felt)
+    (h₁ : state.felts name = some x)
+    (hab : step state program ≠ step state (Sequence branch program))
+    (hhh : (state, none) ≠ step state branch) :
+    Cirgen.step state (.Sequence (.If (Variable.mk name) branch) program)
+  = if (x == 0)
+      then Cirgen.step state program
+      else Cirgen.step state (.Sequence branch program) := by
+  simp only [beq_iff_eq]
+  let a := step state program
+  let b := step state (Sequence branch program)
+  have ha : a = step state program := by simp only
+  have hb : b = step state (Sequence branch program) := by simp only
+  rw [← ha]
+  rw [← hb]
+  by_cases x = 0
+  have hh := (@Ne.ite_eq_left_iff (State × Option Prop) (x = 0) _ a b hab).2 h
+  rw [hh]
+  conv =>
+    lhs
+    unfold step
+    unfold step
+  simp only [beq_iff_eq, Map.update]
+  rw [h₁]
+  simp only
+  have hh₁ := (@Ne.ite_eq_left_iff (State × Option Prop) (x = 0) _ (state, none) (step state branch) hhh).2 h
+  rw [hh₁]
+  simp only
+  conv =>
+    rhs
+    unfold step
+  simp only [beq_iff_eq, Map.update]
+  rw [←ite_not]
+  have hba : b ≠ a := by
+    rw [ha]
+    rw [hb]
+    rw [ne_comm]
+    exact hab
+  have hh := (@Ne.ite_eq_left_iff (State × Option Prop) (¬x = 0) _ b a hba).2 h
+  rw [hh]
+  conv =>
+    lhs
+    unfold step
+    unfold step
+  simp only [beq_iff_eq, Map.update]
+  rw [h₁]
+  simp only
+  rw [←ite_not]
+  have hhhh : step state branch ≠ (state, none) := by
+    rw [ne_comm]
+    exact hhh
+  have hh₁ := (@Ne.ite_eq_left_iff (State × Option Prop) (¬x = 0) _ (step state branch) (state, none) hhhh).2 h
+  rw [hh₁]
+  simp only
+  conv =>
+    rhs
+    unfold step
+  simp only [beq_iff_eq, Map.update]
+  conv in (step (step state branch).fst program) =>
+    unfold step
+  simp only [beq_iff_eq, Map.update]
+
+lemma Cirgen.step_If_collapsible
+    {state : State}
+    {name : String}
+    {branch : Cirgen}
+    (x : Felt)
+    (h₁ : state.felts name = some x) :
+    Cirgen.step state (.If (Variable.mk name) branch)
+  = if (x == 0)
+      then (state, none)
+      else Cirgen.step state branch := by
+  sorry
+
 theorem is0OriginalProgram_constraints_are_what_we_expect :
   ∀ x y z : Felt, (is0OriginalProgram x y z).1.constraints.foldr And _root_.True ↔ (x = 0 ∧ x * x⁻¹ - 1 = 0) := by
   intros x y z
-  apply Iff.intro
-  intros h
-  unfold is0OriginalProgram at h
+  unfold is0OriginalProgram
+  rw [Cirgen.step_Sequence_Assign_collapsible]
+  simp only [State.update, Map.empty, Map.fromList, Map.update, beq_iff_eq]
+  unfold Op.eval
+  simp only
+  rw [Cirgen.step_Sequence_Assign_collapsible]
+  simp only [State.update, Map.empty, Map.fromList, Map.update, beq_iff_eq]
+  unfold Op.eval
+  simp only
+  rw [Cirgen.step_Sequence_Assign_collapsible]
+  simp only [State.update, Map.empty, Map.fromList, Map.update, beq_iff_eq]
+  unfold Op.eval
+  simp only [List.getD_cons_zero, ite_false, ite_true, beq_iff_eq, ne_eq]
+  rw [Cirgen.step_Sequence_Set_collapsible [y, z] (if x = 0 then 1 else 0)]
+  simp only
+  rw [Cirgen.step_Sequence_Assign_collapsible]
+  simp only [State.update, Map.empty, Map.fromList, Map.update, beq_iff_eq]
+  unfold Op.eval
+  simp only
+  rw [Cirgen.step_Sequence_Set_collapsible [y, z] (if (x == 0) = true then 0 else x⁻¹)]
+  simp only [beq_iff_eq, Map.update, List.set_succ, ne_eq]
+  rw [Cirgen.step_Sequence_Assign_collapsible]
+  simp only [State.update, Map.empty, Map.fromList, Map.update, beq_iff_eq]
+  unfold Op.eval
+  simp only [ite_true, ite_false, List.getD_cons_zero, ne_eq]
+  rw [Cirgen.step_Sequence_If_collapsible y]
+  rw [Cirgen.step_Sequence_Assign_collapsible]
+  simp only [State.update, Map.empty, Map.fromList, Map.update, beq_iff_eq]
+  unfold Op.eval
+  simp only
+  rw [Cirgen.step_If_collapsible (1 - y)]
+  simp only [beq_iff_eq, ne_eq]
+  rw [Cirgen.step_Sequence_Assign_collapsible]
+  simp only [State.update, Map.empty, Map.fromList, Map.update, beq_iff_eq]
+  unfold Op.eval
+  simp only
+  rw [Cirgen.step_Sequence_Assign_collapsible]
+  simp only [State.update, Map.empty, Map.fromList, Map.update, beq_iff_eq]
+  unfold Op.eval
+  simp only
+  rw [Cirgen.step_Sequence_Assign_collapsible]
+  simp only [State.update, Map.empty, Map.fromList, Map.update, beq_iff_eq]
+  unfold Op.eval
+  simp only
+  sorry
+  sorry
+  sorry
+  sorry
+  sorry
+  sorry
+  sorry
   sorry
   sorry
 
